Proved transitivity
git-archimport-id: r.oconnor@cs.ru.nl--Nijmegen/CoRN--integration--0--patch-2

model/metric2/L1metric.v
@@ -4,14 +4,40 @@ Require Import CornTac.
 Require Import Qauto.
 Require Import Qabs.
 Require Import QMinMax.
+Require Import Qordfield.
+Require Import COrdFields.
 
 Set Implicit Arguments.
 Record OpenUnit:={OpenUnitasQ:> Q;
 OpenUnitprf:0<OpenUnitasQ/\OpenUnitasQ<1}.
 
 Notation "'ou' x":=(@Build_OpenUnit x (conj (refl_equal Lt) (refl_equal Lt))) (at level 60, no associativity).
-Require Import Qordfield.
-Require Import COrdFields.
+
+Lemma OpenUnit_0_lt : forall (a:OpenUnit), 0 < a.
+intros [a [H0 H1]]; assumption.
+Qed.
+
+Lemma OpenUnit_lt_1 : forall (a:OpenUnit), a < 1.
+intros [a [H0 H1]]; assumption.
+Qed.
+
+Lemma OpenUnit_0_lt_Dual : forall (a:OpenUnit), 0 < 1-a.
+intros [a [H0 H1]].
+simpl.
+rewrite Qlt_minus_iff in H1.
+assumption.
+Qed.
+
+Lemma OpenUnit_Dual_lt_1 : forall (a:OpenUnit), 1-a < 1.
+intros [a [H0 H1]].
+simpl.
+rewrite Qlt_minus_iff.
+replace RHS with a by ring.
+assumption.
+Qed.
+
+Hint Resolve OpenUnit_0_lt OpenUnit_lt_1 OpenUnit_0_lt_Dual OpenUnit_Dual_lt_1.
+
 Definition OpenUnitMult (a b:OpenUnit):OpenUnit.
 intros a b.
 exists (a * b).
@@ -93,6 +119,12 @@ Inductive StepF(X:Type):Type:=
 Definition test1:=(leaf 1). 
 Definition test2:=(glue (ou 1/2) (leaf 0) (leaf 1)).
 
+Fixpoint Mirror (X:Type) (s:StepF X) : StepF X :=
+match s with
+| leaf x => leaf x
+| glue a s1 s2 => glue (OpenUnitDual a) (Mirror s2) (Mirror s1)
+end.
+
 Definition Map(X Y:Type):(X->Y)->(StepF X)->(StepF Y).
 fix 4. intros X Y f [x| a t1 t2].
  exact (leaf (f x)).
@@ -160,32 +192,471 @@ Eval compute in (L1Ball (1#1)%Qpos test2 test1).
 Definition Mesh (X:Type):(StepF X)->Q:=(StepFfold (fun x => 1)(fun b x y => (Qmax (b*x) ((1-b)*y)))).
 Eval compute in (Mesh test2).
 
+Lemma Split_ind : forall X s a (P:StepF X*StepF X -> Prop),
+ (P (SplitL s a,SplitR s a)) -> P (Split s a).
+Proof.
+intros X s a P.
+unfold SplitL, SplitR.
+destruct (Split s a).
+auto with *.
+Qed.
+
+Lemma SplitLR_glue_ind : forall X s1 s2 (a b:OpenUnit) (P:(StepF X) -> (StepF X) -> Prop),
+ (forall (H:a < b), P (SplitL s1 (OpenUnitDiv a b H)) (glue (OpenUnitAux b a H) (SplitR s1 (OpenUnitDiv a b H)) s2)) ->
+ (forall (H:b < a), P (glue (OpenUnitDiv b a H) s1 (SplitL s2 (OpenUnitAux a b H))) (SplitR s2 (OpenUnitAux a b H))) ->
+ (a == b -> P s1 s2) ->
+ P (SplitL (glue b s1 s2) a) (SplitR (glue b s1 s2) a).
+Proof.
+intros X s1 s2 a b P Hl Hr Heq.
+unfold SplitL, SplitR.
+simpl.
+destruct (Q_dec a b) as [[Hab|Hab]|Hab]; 
+ try apply Split_ind; simpl; auto with *.
+Qed.
+
+Lemma SplitL_glue_ind : forall X s1 s2 (a b:OpenUnit) (P:(StepF X) -> Prop),
+ (forall (H:a < b), P (SplitL s1 (OpenUnitDiv a b H))) ->
+ (forall (H:b < a), P (glue (OpenUnitDiv b a H) s1 (SplitL s2 (OpenUnitAux a b H)))) ->
+ (a == b -> P (s1)) ->
+ P (SplitL (glue b s1 s2) a).
+Proof.
+intros.
+apply (SplitLR_glue_ind s1 s2 a b (fun a b => P a));
+assumption.
+Qed.
+
+Lemma SplitR_glue_ind : forall X s1 s2 (a b:OpenUnit) (P:(StepF X) -> Prop),
+ (forall (H:a < b), P (glue (OpenUnitAux b a H) (SplitR s1 (OpenUnitDiv a b H)) s2)) ->
+ (forall (H:b < a), P (SplitR s2 (OpenUnitAux a b H))) ->
+ (a == b -> P (s2)) ->
+ P (SplitR (glue b s1 s2) a).
+Proof.
+intros.
+apply (SplitLR_glue_ind s1 s2 a b (fun a b => P b));
+assumption.
+Qed.
+
+Fixpoint StepF_Qeq (X:Type) (s1 s2: StepF X) : Prop :=
+match s1, s2 with
+|leaf x, leaf y => x = y
+|glue a x1 x2, glue b y1 y2 => a == b /\ (StepF_Qeq x1 y1) /\ (StepF_Qeq x2 y2)
+|_, _ => False
+end.
+
+Lemma StepF_Qeq_refl : forall X (s: StepF X), StepF_Qeq s s.
+Proof.
+induction s; simpl; auto with *.
+Qed.
+
+Lemma StepF_Qeq_sym : forall X (s t: StepF X), StepF_Qeq s t -> StepF_Qeq t s.
+Proof.
+induction s; induction t; try contradiction; simpl; auto with *.
+intros [H0 [H1 H2]].
+repeat split; eauto with *.
+Qed.
+
+Lemma StepF_Qeq_trans : forall X (s t u: StepF X), StepF_Qeq s t -> StepF_Qeq t u -> StepF_Qeq s u.
+Proof.
+induction s; induction t; induction u; try contradiction; simpl; auto with *.
+ intros; transitivity x0; assumption.
+intros [H0 [H1 H2]] [H3 [H4 H5]].
+repeat split; eauto with *.
+Qed.
+
+Hint Resolve StepF_Qeq_refl StepF_Qeq_sym StepF_Qeq_trans.
+
+Lemma Mirror_resp_Qeq : forall X (s t:StepF X), StepF_Qeq s t -> StepF_Qeq (Mirror s) (Mirror t).
+Proof.
+induction s; induction t; intros Hst; simpl in *; try assumption; try contradiction.
+destruct Hst as [Ho [Hst1 Hst2]].
+repeat split.
+  rewrite Ho; reflexivity.
+ apply IHs2; assumption.
+apply IHs1; assumption.
+Qed.
+
+Hint Resolve Mirror_resp_Qeq.
+
+Lemma MirrorMirror : forall X (s:StepF X), (StepF_Qeq (Mirror (Mirror s)) s).
+Proof.
+induction s.
+ simpl; reflexivity.
+repeat split; auto with *.
+simpl; ring.
+Qed.   
+
+Hint Resolve MirrorMirror.
+
+Lemma SplitR_resp_Qeq : forall X (s t:StepF X) (a b:OpenUnit), a == b -> StepF_Qeq s t -> StepF_Qeq (SplitR s a) (SplitR t b).
+Proof.
+induction s; induction t; intros a b Hab Hst; simpl in *; try assumption; try contradiction.
+destruct Hst as [Ho [Hst1 Hst2]].
+apply SplitR_glue_ind; intros Hao; apply SplitR_glue_ind; intros Hbo; repeat split; auto with *;
+ try solve [elim (Qlt_not_le _ _ Hao); rewrite Hab; rewrite Ho; try rewrite Hbo; auto with *
+           |elim (Qlt_not_le _ _ Hbo); rewrite <- Hab; rewrite <- Ho; try rewrite Hao; auto with *];
+ try apply IHs1; try apply IHs2; auto with *; simpl; try (rewrite Hab; rewrite Ho; reflexivity).
+Qed.
+
+Hint Resolve SplitR_resp_Qeq.
+
+Lemma MirrorSplitL : forall X (s:StepF X) (a b:OpenUnit), b == (OpenUnitDual a) -> (StepF_Qeq (Mirror (SplitL s a)) (SplitR (Mirror s) b)).
+Proof.
+induction s.
+ auto with *.
+intros a b Hab; simpl in Hab.
+simpl.
+apply SplitL_glue_ind; intros Hao; apply SplitR_glue_ind; intros Hoa; simpl in Hoa;
+ try (repeat split; auto with *; try apply IHs1; try apply IHs2; simpl; rewrite Hab; field; auto with *).
+      elim (Qlt_not_le _ _ Hao).
+      rewrite Qlt_minus_iff in Hoa.
+      rewrite Qle_minus_iff.
+      replace RHS with (1 - o + - (1 - a)) by ring.
+      rewrite <- Hab.
+      auto with *.
+     elim (Qlt_not_le _ _ Hao).
+     rewrite Qle_minus_iff.
+     replace RHS with (1 - o + - (1 - a)) by ring.
+     rewrite <- Hab.
+     rewrite <- Hoa.
+     ring_simplify.
+     auto with *.
+    intros H; ring_simplify in H.
+    revert H; change (~(a==0)); auto with *.
+   elim (Qlt_not_le _ _ Hao).
+   rewrite Qle_minus_iff.
+   rewrite Qlt_minus_iff in Hoa.
+   replace RHS with (1 - a + - (1 - o)) by ring.
+   rewrite <- Hab.
+   auto with *.
+  elim (Qlt_not_le _ _ Hao).
+  rewrite Qle_minus_iff.
+  replace RHS with (1 - a + - (1 - o)) by ring.
+  rewrite <- Hab.
+  rewrite <- Hoa.
+  ring_simplify.
+  auto with *.
+ elim (Qlt_not_le _ _ Hoa).
+ rewrite Hab.
+ rewrite Hao.
+ auto with *.
+elim (Qlt_not_le _ _ Hoa).
+rewrite Hab.
+rewrite Hao.
+auto with *.
+Qed.
+
+Lemma MirrorSplitR : forall X (s:StepF X) (a b:OpenUnit), b == (OpenUnitDual a) -> (StepF_Qeq (Mirror (SplitR s a)) (SplitL (Mirror s) b)).
+Proof.
+intros X s a b H.
+apply StepF_Qeq_trans with (Mirror (SplitR (Mirror (Mirror s)) a));
+ auto with *.
+apply StepF_Qeq_trans with (Mirror (Mirror (SplitL (Mirror s) b)));
+ auto with *.
+apply Mirror_resp_Qeq.
+apply StepF_Qeq_sym.
+apply MirrorSplitL.
+simpl in *.
+rewrite H.
+ring.
+Qed.
+
+Lemma SplitL_resp_Qeq : forall X (s t:StepF X) (a b:OpenUnit), a == b -> StepF_Qeq s t -> StepF_Qeq (SplitL s a) (SplitL t b).
+Proof.
+intros X s t a b H H0.
+apply StepF_Qeq_trans with (Mirror (Mirror (SplitL s a)));
+ auto with *.
+apply StepF_Qeq_trans with (Mirror (SplitR (Mirror s) (OpenUnitDual a))).
+ apply Mirror_resp_Qeq.
+ apply MirrorSplitL; auto with *.
+apply StepF_Qeq_trans with (Mirror (SplitR (Mirror t) (OpenUnitDual b))).
+ apply Mirror_resp_Qeq.
+ apply SplitR_resp_Qeq; auto with *.
+ simpl; rewrite H; reflexivity.
+apply StepF_Qeq_trans with (Mirror (Mirror (SplitL t b)));
+ auto with *.
+apply Mirror_resp_Qeq.
+apply StepF_Qeq_sym.
+apply MirrorSplitL; auto with *.
+Qed.
+
+Hint Resolve SplitL_resp_Qeq.
+
+Lemma SplitLSplitL : forall X (s:StepF X) (a b c:OpenUnit), (a*b==c) -> 
+ (StepF_Qeq (SplitL (SplitL s a) b) (SplitL s c)).
+Proof.
+induction s.
+ intros a b c _.
+ apply StepF_Qeq_refl.
+intros a b c H.
+apply SplitL_glue_ind; intros Hao.
+  apply SplitL_glue_ind; intros Hco.
+    apply IHs1.
+    simpl.
+    rewrite <- H; field.
+    auto with *.
+   elim (Qlt_not_le a c).
+    apply Qlt_trans with o; assumption.
+   rewrite <- H.
+   replace RHS with (1*a) by ring.
+   replace LHS with (b*a) by ring.
+   apply Qmult_le_compat_r; auto with *.
+  elim (Qlt_not_le a c).
+   rewrite Hco.
+   apply Qlt_le_trans with o; auto with *.
+  rewrite <- H.
+  replace RHS with (1*a) by ring.
+  replace LHS with (b*a) by ring.
+  apply Qmult_le_compat_r; auto with *.
+ apply SplitL_glue_ind; intros Hbd.
+   apply SplitL_glue_ind; intros Hco.
+     apply SplitL_resp_Qeq; auto with *.
+     simpl.
+     rewrite <- H.
+     field; auto with *.
+    elim (Qlt_not_le _ _ Hbd).
+    simpl.
+    apply Qle_shift_div_r; auto with *.
+    rewrite Qmult_comm; rewrite  H; auto with *.
+   elim (Qlt_not_le _ _ Hbd).
+   simpl.
+   apply Qle_shift_div_r; auto with *.
+   rewrite Qmult_comm; rewrite H; rewrite Hco; auto with *.
+  apply SplitL_glue_ind; intros Hco.
+    elim (Qlt_not_le _ _ Hbd).
+    simpl.
+    apply Qle_shift_div_l; auto with *.
+    rewrite Qmult_comm; rewrite  H; auto with *.
+   repeat split; auto with *.
+    simpl.
+    rewrite <- H.
+    field; auto with *.
+   apply IHs2.
+   simpl.
+   rewrite <- H.
+   field; repeat split; auto with *.
+   clear - Hao; rewrite Qlt_minus_iff in Hao.
+   auto with *.
+  elim (Qlt_not_le _ _ Hbd).
+  simpl.
+  apply Qle_shift_div_l; auto with *.
+  rewrite Qmult_comm; rewrite H; auto with *.
+ assert (Y:o==c).
+  rewrite <- H.
+  rewrite Hbd.
+  simpl.
+  field.
+  auto with *.
+ apply SplitL_glue_ind; intros Hco;
+  try (elim (Qlt_not_le _ _ Hco); rewrite Y; auto with *).
+ auto with *.
+apply SplitL_glue_ind; intros Hco.
+  apply SplitL_resp_Qeq; auto with *.
+  simpl.
+  rewrite <- H.
+  rewrite Hao.
+  field; auto with *.
+ elim (Qlt_not_le _ _ Hco).
+ rewrite <- H.
+ rewrite <- Hao.
+ replace RHS with (1*a) by ring.
+ replace LHS with (b*a) by ring.
+ apply Qmult_le_compat_r; auto with *.
+elim (Qlt_not_le b 1).
+ auto with *.
+rewrite <- Hao in Hco.
+rewrite Hco in H.
+apply Qmult_lt_0_le_reg_r with a.
+ auto with *.
+ring_simplify.
+rewrite H.
+auto with *.
+Qed.
+
+Lemma SplitRSplitR : forall X (s:StepF X) (a b c:OpenUnit), (a+b-a*b==c) -> 
+ (StepF_Qeq (SplitR (SplitR s a) b) (SplitR s c)).
+Proof.
+intros X s a b c H.
+apply StepF_Qeq_trans with (Mirror (Mirror (SplitR (SplitR s a) b)));
+ auto with *.
+apply StepF_Qeq_trans with (Mirror (Mirror (SplitR s c)));
+ auto with *.
+apply Mirror_resp_Qeq.
+apply StepF_Qeq_trans with (SplitL (SplitL (Mirror s) (OpenUnitDual a)) (OpenUnitDual b)).
+ apply StepF_Qeq_trans with (SplitL (Mirror (SplitR s a)) (OpenUnitDual b)).
+  apply MirrorSplitR; auto with *.
+ apply SplitL_resp_Qeq; auto with *.
+ apply MirrorSplitR; auto with *.
+apply StepF_Qeq_trans with (SplitL (Mirror s) (OpenUnitDual c)).
+ apply SplitLSplitL.
+ simpl.
+ rewrite <- H.
+ ring.
+apply StepF_Qeq_sym.
+apply MirrorSplitR; auto with *.
+Qed.
+
+Lemma SplitLSplitR : forall X (s:StepF X) (a b c d:OpenUnit), (a+b-a*b==c) -> (d*c==a) -> 
+ (StepF_Qeq (SplitL (SplitR s a) b) (SplitR (SplitL s c) d)).
+Proof.
+induction s.
+ intros a b c d _ _.
+ apply StepF_Qeq_refl.
+intros a b c d H0 H1.
+apply SplitR_glue_ind; intros Hao.
+  assert (Hao':~ o - a == 0).
+   intros H.
+   elim (Qlt_not_le _ _ Hao).
+   rewrite Qle_minus_iff.
+   replace RHS with (- (o- a)) by ring.
+   rewrite H.
+   auto with *.
+  apply SplitL_glue_ind; intros Hbz; simpl in Hbz.
+    apply SplitL_glue_ind; intros Hco.
+      apply IHs1; simpl; [rewrite <- H0|rewrite <- H1]; field; auto with *.
+     elim (Qlt_not_le _ _ Hbz).
+     rewrite Qlt_minus_iff in Hco.
+     rewrite Qle_minus_iff.
+     replace RHS with ((a + b - a*b + -o)/(1 -a)) by (field; auto with *).
+     rewrite H0.
+     apply Qle_shift_div_l; auto with *.
+     replace LHS with 0 by ring.
+     auto with *.
+    elim (Qlt_not_le _ _ Hbz).
+    rewrite Qle_minus_iff.
+    replace RHS with ((a + b - a*b + -o)/(1 -a)) by (field; auto with *).
+    rewrite H0.
+    rewrite Hco.
+    replace RHS with 0 by (field; auto with *).
+    auto with *.
+   apply SplitL_glue_ind; intros Hco.
+     elim (Qlt_not_le _ _ Hbz).
+     rewrite Qlt_minus_iff in Hco.
+     rewrite Qle_minus_iff.
+     replace RHS with ((o + -(a + b - a*b))/(1 -a)) by (field; auto with *).
+     rewrite H0.
+     apply Qle_shift_div_l; auto with *.
+     replace LHS with 0 by ring.
+     auto with *.
+    apply SplitR_glue_ind; intros Hdz; simpl in Hdz.
+      repeat split; simpl.
+        field_simplify; auto with *.
+        rapply Qmult_simpl.
+         rewrite <- H1; ring.
+        apply Qinv_comp.
+        replace LHS with (a + b - a*b - a) by ring.
+        rewrite H0.
+        replace RHS with (c - (d*c)) by ring.
+        rewrite H1.
+        reflexivity.
+       apply SplitR_resp_Qeq; auto with *; simpl.
+       rewrite <- H1; field; auto with *.
+      apply SplitL_resp_Qeq; auto with *; simpl.
+      rewrite <- H0; field; auto with *.
+     elim (Qlt_not_le _ _ Hdz).
+     apply Qle_shift_div_l; auto with *.
+     rewrite H1; auto with *.
+    elim (Qlt_not_le _ _ Hao).
+    rewrite <- H1.
+    rewrite Hdz.
+    replace RHS with (o:Q) by (field; auto with *).
+    auto with *.
+   elim (Qlt_not_le _ _ Hbz).
+   rewrite <- Hco.
+   rewrite <- H0.
+   replace RHS with (b:Q) by (field; auto with *).
+   auto with *.
+  apply SplitL_glue_ind; intros Hco.
+    elim (Qlt_not_le _ _ Hco).
+    rewrite <- H0.
+    rewrite Hbz.
+    replace RHS with (o:Q) by (field; auto with *).
+    auto with *.
+   elim (Qlt_not_le _ _ Hco).
+   rewrite <- H0.
+   rewrite Hbz.
+   replace LHS with (o:Q) by (field; auto with *).
+   auto with *.
+  apply SplitR_resp_Qeq; simpl; auto with *.
+  rewrite <- H1.
+  rewrite Hco.
+  field; auto with *.
+ apply SplitL_glue_ind; intros Hco.
+   elim (Qlt_not_le _ _ Hco).
+   rewrite <- H0.
+   apply Qlt_le_weak.
+   rewrite Qlt_minus_iff in *.
+   replace RHS with (a + - o + b*(1-a)) by ring.
+   assert (Z:0 < (1-a)) by auto with *.
+   Qauto_pos.
+  assert (Hco':~ c - o == 0).
+   intros H.
+   elim (Qlt_not_le _ _ Hco).
+   rewrite Qle_minus_iff.
+   replace RHS with (- (c- o)) by ring.
+   rewrite H.
+   auto with *.
+  apply SplitR_glue_ind; intros Hdz; simpl in Hdz.
+    elim (Qlt_not_le _ _ Hdz).
+    apply Qle_shift_div_r; auto with *.
+    rewrite H1; auto with *.
+   apply IHs2; simpl; [rewrite <- H0|rewrite <- H1]; field; auto with *.
+  elim (Qlt_not_le _ _ Hao).
+  rewrite <- H1.
+  rewrite Hdz.
+  replace LHS with (o:Q) by (field; auto with *).
+  auto with *.
+ elim (Qlt_not_le _ _ Hao).
+ rewrite <- H1.
+ rewrite <- Hco.
+ rewrite Qle_minus_iff.
+ replace RHS with (c * (1-d)) by ring.
+ apply Qlt_le_weak.
+ assert (Z:0 < (1-d)) by auto with *.
+ Qauto_pos.
+apply SplitL_glue_ind; intros Hco.
+  elim (Qlt_not_le _ _ Hco).
+  rewrite <- Hao.
+  rewrite <- H1.
+  rewrite Qle_minus_iff.
+  replace RHS with (c * (1-d)) by ring.
+  apply Qlt_le_weak.
+  assert (Z:0 < (1-d)) by auto with *.
+  Qauto_pos.
+ apply SplitR_glue_ind; intros Hdz; simpl in Hdz.
+   elim (Qlt_not_le _ _ Hdz).
+   apply Qle_shift_div_r; auto with *.
+   rewrite <- Hao.
+   rewrite H1; auto with *.
+  elim (Qlt_not_le _ _ Hdz).
+  apply Qle_shift_div_l; auto with *.
+  rewrite <- Hao.
+  rewrite H1; auto with *.
+ apply SplitL_resp_Qeq; simpl; auto with *.
+ rewrite <- H0.
+ rewrite <- Hao.
+ field; auto with *.
+elim (Qlt_not_le (d*c) a).
+ rewrite Hao.
+ rewrite Hco.
+ rewrite Qlt_minus_iff.
+ replace RHS with (o * (1-d)) by ring.
+ assert (Z:0 < (1-d)) by auto with *.
+ Qauto_pos.
+rewrite H1.
+auto with *.
+Qed.
+
 Require Import Setoid.
 Section Equivalence.
 Variable X:Type.
 Variable Xeq:X->X->Prop.
 Hypothesis Xst:(Setoid_Theory X Xeq).
 Hint Resolve (Seq_trans X Xeq Xst) (Seq_sym X Xeq Xst) (Seq_refl X Xeq Xst):foo.
-Print Setoid_Theory.
 
 Definition StepFfoldProp:=StepFfold (fun x => x ) (fun _ a b => a /\ b ).
 
 Definition StepF_eq (f g:StepF X):Prop:=
-( StepFfoldProp (Map2 Xeq f g)).
-(*
-Fixpoint StepFfoldProp (s : StepF Prop) {struct s} : Prop :=
-  match s with
-  | leaf x => x
-  | glue _ t1 t2 => (StepFfoldProp t1)/\ (StepFfoldProp t2)
-  end.
-
-Definition StepF_eq (f g:StepF X):Prop:=
-( (fix StepFfoldProp (s : StepF Prop) {struct s} : Prop :=
-  match s with
-  | leaf x => x
-  | glue _ t1 t2 => (StepFfoldProp t1)/\ (StepFfoldProp t2)
-  end) (Map2 Xeq f g)).
-*)
+(StepFfoldProp (Map2 Xeq f g)).
 
 Hint Unfold StepFfoldProp StepFfold StepF_eq.
 Lemma Qdec_eq_ind: forall a b:Q, forall P:{a<b}+{b<a}+{a==b}->Type,
@@ -198,7 +669,7 @@ intros a b P H H1 [[H2|H2]|H2].
 auto with *.
 Qed.
 
-Notation "x === y" := (StepF_eq x y) (at level 100).
+Notation "x === y" := (StepF_eq x y) (at level 60).
 
 Lemma StepF_eq_refl:forall x : StepF X, x === x.
 intro s.
@@ -209,7 +680,30 @@ Qed.
 
 Hint Resolve StepF_eq_refl:sfarith.
 
-Print Setoid_Theory.
+Lemma StepF_eq_aux:forall s s1 s2, forall a, s1 === (SplitL s a) -> s2 === (SplitR s a) -> (glue a s1 s2) === s.
+intros s s1 s2 a. unfold SplitL, SplitR, StepF_eq. simpl. 
+intros.
+destruct (Split s a) as [s3 s4].
+split; assumption.
+Qed.
+
+Lemma StepF_Qeq_eq : forall s t, (StepF_Qeq s t) -> s === t.
+Proof.
+induction s; induction t; try contradiction; simpl.
+ intros H.
+ rewrite H.
+ auto with *.
+intros [H [H0 H1]].
+apply StepF_eq_aux.
+ apply IHs1.
+ apply SplitL_glue_ind; intros H2;
+  try (elim (Qlt_not_le _ _ H2); rewrite H); auto with *.
+apply IHs2.
+apply SplitR_glue_ind; intros H2;
+ try (elim (Qlt_not_le _ _ H2); rewrite H); auto with *.
+Qed.
+
+(*
 Lemma glue_resp_Qeq:forall s t:StepF X, forall a b:OpenUnit, a==b -> (StepF_eq (glue a s t) (glue b s t)).
 intros s t a b H.
 unfold StepF_eq; simpl.
@@ -217,21 +711,31 @@ elim (Q_dec a b) using Qdec_eq_ind;auto with *.
 intros H1.
 change ((StepF_eq s s) /\ (StepF_eq t t)); auto with *.
 Qed.
-
-Lemma StepF_eq_aux:forall s s1 s2, forall a, (StepF_eq s1 (fst (Split s a))) -> (StepF_eq s2 (snd (Split s a))) ->(StepF_eq (glue a s1 s2) s).
-intros s s1 s2 a. unfold StepF_eq. simpl. 
-intros.
-destruct (Split s a) as [s3 s4].
-simpl in *. auto with *.
+*)
+Lemma glue_wd:forall (s1 s2 t1 t2:StepF X) (a b:OpenUnit), a==b -> s1 === s2 -> t1 === t2 -> ((glue a s1 t1) === (glue b s2 t2)).
+Proof.
+intros s1 s2 t1 t2 a b Hab Hs Ht.
+unfold StepF_eq; simpl.
+elim (Q_dec a b) using Qdec_eq_ind;auto with *.
 Qed.
 
+Lemma glue_eq_ind : forall s1 s2 s a (P:Prop), (s1 === (SplitL s a) -> s2 === (SplitR s a) -> P) -> (glue a s1 s2 === s) -> P.
+Proof.
+intros s1 s2 s a P H H0.
+unfold SplitL, SplitR, StepF_eq in *.
+simpl in *.
+destruct (Split s a).
+destruct H0.
+apply H; assumption.
+Qed.
 
+Hint Resolve StepF_eq_aux glue_wd :starith.
 
-Hint Resolve StepF_eq_aux glue_resp_Qeq:starith.
 Lemma glueSplit_eq:forall s:StepF X, forall a:OpenUnit, 
- (glue a (fst (Split s a)) (snd (Split s a))) === s.
+ (glue a (SplitL s a) (SplitR s a)) === s.
 auto with *.
 Qed.
+
 
 Lemma Mapleaf(Y:Type): forall f:X->Y, 
   forall x, (Map f (leaf x))=(leaf (f x)).
@@ -253,17 +757,19 @@ rewrite IHs2. destruct (Split s2 (OpenUnitAux a o H0)). auto with *.
 auto.
 Qed.
 
-Lemma fstsplitmap(Y:Type): forall x:(StepF X), forall a, forall f:X->Y, 
-    fst (Split (Map f x) a) = Map f (fst (Split x a)).
-intros. rewrite splitmap. destruct (Split x a). simpl. auto.
+Lemma SplitLMap(Y:Type): forall x:(StepF X), forall a, forall f:X->Y, 
+    SplitL (Map f x) a = Map f (SplitL x a).
+intros. unfold SplitL. rewrite splitmap. destruct (Split x a). simpl. auto.
 Qed.
 
-Lemma sndsplitmap(Y:Type): forall x:(StepF X), forall a, forall f:X->Y, 
+Lemma SplitRMap(Y:Type): forall x:(StepF X), forall a, forall f:X->Y, 
     snd (Split (Map f x) a) = Map f (snd (Split x a)).
-intros. rewrite splitmap. destruct (Split x a). simpl. auto.
+intros. unfold SplitR. rewrite splitmap. destruct (Split x a). simpl. auto.
 Qed.
 
 End  Equivalence.
+
+Hint Resolve StepF_eq_refl StepF_Qeq_eq splitmap SplitLMap SplitRMap:foo.
 Section Equivalence1.
 Variable X:Type.
 Variable Xeq:X->X->Prop.
@@ -278,9 +784,8 @@ Print StepF_eq.
 
 Add Setoid X Xeq Xst as Xth.
 
-Hint Resolve splitmap fstsplitmap sndsplitmap:foo.
 Hint Unfold StepFfoldProp StepFfold StepF_eq.
-Lemma map_resp_StepF_eq: forall f:X->Y, 
+Lemma Map_resp_StepF_eq: forall f:X->Y, 
     (forall x y, (Xeq x y)-> (Yeq (f x) (f y))) ->
     forall s t:(StepF X), (s === t) -> (StepF_eq Yeq (Map f s) (Map f t)).
 intros f H.
@@ -336,6 +841,7 @@ Add Setoid X Xeq Xst as Xth1.
 Hint Resolve (Seq_trans X Xeq Xst) (Seq_sym X Xeq Xst) (Seq_refl X Xeq Xst):foo.
 Notation "x === y" := (StepF_eq Xeq x y) (at level 60).
 
+
 (* Add Setoid X Xeq Xst as Xth.*)
 Lemma StepFfoldPropglue:forall y o,
  StepFfoldProp (glue o (fst (Split y o)) (snd (Split y o))) <->
@@ -364,7 +870,7 @@ simpl.
 reflexivity.
 Qed.
 
-Hint Resolve splitmap fstsplitmap sndsplitmap StepFfoldPropglue:foo.
+Hint Resolve StepFfoldPropglue:foo.
 Lemma StepFfoldProp_morphism:forall x y:(StepF Prop),
   (StepF_eq iff x y) ->
   ((StepFfoldProp x)<->(StepFfoldProp y)).
@@ -387,17 +893,116 @@ o)))))).
 auto with *.
 Qed.
 
-(*
-The next goal:
+Lemma StepF_eq_resp_Qeq : forall s t u v, (StepF_Qeq s t) -> (StepF_Qeq u v) -> s === u -> t === v.
+Proof.
+induction s; induction t; try contradiction.
+ intros u v Hst Huv Hsu.
+ simpl in Hst.
+ unfold StepF_eq in *.
+ simpl in *.
+ rewrite <- Hst.
+ rewrite <- (StepFfoldProp_morphism (Map (Xeq x) u)); auto with *.
+ apply (Map_resp_StepF_eq Xst); auto with *.
+  split;[apply iff_refl|apply iff_sym|apply iff_trans].
+ intros a b Hab; split; eauto with *.
+intros u v [H [Hst0 Hst1]] Huv Hsu.
+destruct Hsu as [Hsu1 Hsu2] using (glue_eq_ind Xeq).
+apply StepF_eq_aux.
+ eapply IHs1.
+   assumption.
+  apply SplitL_resp_Qeq.
+   apply H.
+  apply Huv.
+ assumption.
+eapply IHs2.
+  assumption.
+ apply SplitR_resp_Qeq.
+  apply H.
+ apply Huv.
+assumption.
+Qed.
 
-Lemma Split_morphism1: forall o a b, a === b ->
-   (fst (Split a o)) === (fst (Split b o)).
-intros o a b H.
- unfold Split. destruct  (Q_dec o o0) as [[H1 | H2]  | H3]; auto with *.
+Lemma Mirror_eq_Mirror : forall s t, Mirror s === Mirror t <-> s === t.
+Proof.
+induction s.
+ induction t; simpl.
+  reflexivity.
+ simpl in *.
+ change (leaf x === (Mirror t2) /\ leaf x === (Mirror t1) <-> leaf x === t1 /\ leaf x === t2).
+ tauto.
+intros t.
+simpl.
+split; apply glue_eq_ind; intros H0 H1.
+ apply StepF_eq_aux.
+  rewrite <- IHs1.
+  eapply StepF_eq_resp_Qeq;[| |apply H1]; auto with *.
+  apply StepF_Qeq_sym.
+  apply MirrorSplitL; auto with *.
+ rewrite <- IHs2.
+ eapply StepF_eq_resp_Qeq;[| |apply H0]; auto with *.
+ apply StepF_Qeq_sym.
+ apply MirrorSplitR; auto with *.
+apply StepF_eq_aux.
+ eapply StepF_eq_resp_Qeq;[apply StepF_Qeq_refl|apply MirrorSplitR; apply Qeq_refl|].
+ rewrite IHs2.
+ assumption.
+eapply StepF_eq_resp_Qeq;[apply StepF_Qeq_refl|apply MirrorSplitL; apply Qeq_refl|].
+rewrite IHs1.
+assumption.
+Qed.
 
-  Not clear how to continue
+Lemma StepFfoldPropSplitL : 
+ forall (s : StepF Prop) a, StepFfoldProp s -> StepFfoldProp (SplitL s a).
+Proof.
+induction s; intros a H.
+ assumption.
+destruct H.
+apply SplitL_glue_ind; intros Hao.
+  apply IHs1; assumption.
+ split.
+  assumption.
+ apply IHs2.
+ assumption.
+assumption.
+Qed.
 
+Lemma SplitL_resp_Xeq : forall s1 s2 a, s1 === s2 -> SplitL s1 a === SplitL s2 a.
+Proof.
+induction s1.
+ intros s2 a H.
+ unfold SplitL at 1.
+ simpl.
+ unfold StepF_eq in *.
+ simpl in *.
+ rewrite <- SplitLMap.
+ apply StepFfoldPropSplitL.
+ assumption.
+intros s2 a H.
+destruct H using (glue_eq_ind Xeq).
+apply SplitL_glue_ind; intros Hao.
+  eapply StepF_eq_resp_Qeq;[| |apply IHs1_1;apply H].
+   apply StepF_Qeq_refl.
+  apply SplitLSplitL.
+  simpl; field; auto with *.
+ apply StepF_eq_aux.
+  eapply StepF_eq_resp_Qeq;[| |apply H]; auto with *.
+  apply StepF_Qeq_sym.
+  apply SplitLSplitL.
+  simpl; field; auto with *.
+ eapply StepF_eq_resp_Qeq;[| |apply IHs1_2; apply H0]; auto with *.
+ apply SplitLSplitR; simpl; field; auto with *.
+eapply StepF_eq_resp_Qeq;[| |apply H]; auto with *.
+Qed.
 
+Lemma SplitR_resp_Xeq : forall s1 s2 a, s1 === s2 -> SplitR s1 a === SplitR s2 a.
+Proof.
+intros s1 s2 a H.
+eapply StepF_eq_resp_Qeq; try (eapply StepF_Qeq_trans;[apply Mirror_resp_Qeq; apply StepF_Qeq_sym; apply MirrorSplitR; reflexivity|apply MirrorMirror]).
+rewrite  Mirror_eq_Mirror.
+apply SplitL_resp_Xeq.
+rewrite Mirror_eq_Mirror.
+assumption.
+Qed.
 End Equivalence2.
 
 Section Equivalence3.
@@ -412,69 +1017,90 @@ Variable Zeq:Z->Z->Prop.
 Hypothesis Zst:(Setoid_Theory Z Zeq).
 Hint Resolve (Seq_trans X Xeq Xst) (Seq_sym X Xeq Xst) (Seq_refl X Xeq Xst):foo.
 Hint Resolve (Seq_trans Y Yeq Yst) (Seq_sym Y Yeq Yst) (Seq_refl Y Yeq Yst):foo.
+
 Lemma Map2_morphism2:forall f, (forall x x' y y',
   (Xeq x x) -> (Yeq y y')-> (Zeq (f x y) (f x' y'))) ->
   forall s t t', (StepF_eq Yeq t t') ->
   (StepF_eq Zeq (Map2 f s t) (Map2 f s t')).
 intros f H.
-induction t. induction t'. 
-   unfold StepF_eq. simpl. unfold StepFfoldProp. simpl.
-   intro Hxx0. induction s.
-    simpl. auto with *.
-    simpl.  elim (Q_dec o o) using Qdec_eq_ind;simpl;auto with *.
- intro. 
- Does not seem like fun.
-
-simpl in H0.
- split; auto with *.
-    apply IHs1.
+induction s.
+ intros t t' H0.
+ simpl.
+ eapply Map_resp_StepF_eq;try apply Yst; auto with *.
+intros t t' H0.
 simpl.
-   unfold Map2; simpl. auto with *.
-  unfold StepF_eq. simpl. unfold StepFfoldProp;simpl;intuition.
-intros y H0.
-unfold StepF_eq in H0. simpl in H0.
-transitivity (StepFfoldProp ((glue o (fst (Split y o)) (snd (Split y 
-o))))).
-  change ((StepFfoldProp x1 /\ StepFfoldProp x2) <->
-  ((StepFfoldProp (fst (Split y o)) /\ (StepFfoldProp (snd (Split y 
-o)))))).
-  destruct (Split y o) as [l r].
-  destruct H0 as [H0l H0r].
-  rewrite (IHx1 l); try assumption.
-  rewrite (IHx2 r); try assumption.
-  simpl.
-  tauto.
-auto with *.
+apply Split_ind.
+apply Split_ind.
+simpl.
+apply StepF_eq_aux.
+ apply SplitL_glue_ind; intros H1; try (elim (Qlt_not_le _ _ H1); auto with *).
+ apply IHs1.
+ apply SplitL_resp_Xeq; auto with *.
+apply SplitR_glue_ind; intros H1; try (elim (Qlt_not_le _ _ H1); auto with *).
+apply IHs2.
+apply SplitR_resp_Xeq; auto with *.
 Qed.
-*)
 
-Axiom PropST:(Setoid_Theory Prop iff).
+Notation "x === y" := (StepF_eq Xeq x y) (at level 60).
 
-Lemma StepF_eq_trans:forall x y z : StepF X, (x === y) -> y === z -> x === z.
+Lemma StepF_eq_trans:forall x y z : StepF X, x === y -> y === z -> x === z.
 induction x. intros.
  unfold StepF_eq;simpl;auto with *.
   cut (StepFfoldProp (Map (Xeq x) y)); try auto.
- rewrite (StepFfoldProp_morphism (Map (Xeq x) y) (Map (Xeq x) z));try auto.
- apply (map_resp_StepF_eq Xst PropST); auto with *.
- intros x0 y0 Hx0y0. rewrite Hx0y0. intuition.
+ intros H1.
+ rewrite <- (StepFfoldProp_morphism Xst (Map (Xeq x) y)); auto with *.
+ eapply Map_resp_StepF_eq; try apply Xst; auto with *.
+  split;[apply iff_refl|apply iff_sym|apply iff_trans].
+ intros a b Hab.
+ split; eauto with *.
 intros.
-unfold StepF_eq. 
-rewrite <- (StepFfoldProp_morphism (Map2 Xeq (glue o x1 x2) y) (Map2 Xeq (glue o x1 x2) z)).
-2:auto with *.
+destruct H using (glue_eq_ind Xeq).
+apply StepF_eq_aux.
+ eapply IHx1.
+  apply H.
+ apply SplitL_resp_Xeq.
+  apply Xst.
+ assumption.
+eapply IHx2.
+ apply H1.
+apply SplitR_resp_Xeq.
+ apply Xst.
+assumption.
+Qed.
 
-fold StepFfoldProp.
+Lemma Map2_morphism1:forall f, (forall x x' y y',
+  (Xeq x x) -> (Yeq y y')-> (Zeq (f x y) (f x' y'))) ->
+  forall t t' s, (StepF_eq Xeq t t') ->
+  (StepF_eq Zeq (Map2 f t s) (Map2 f t' s)).
+intros f H.
+induction t.
+ induction t'.
 
-revert H.
-unfold StepF_eq. simpl. 
-(*rewrite (StepFfoldProp_morphism (Map2 iff (Map2 Xeq (glue o x1 x2) y) (Map2 Xeq (glue o x1 x2) z))
-                  ((Map2 Xeq (glue o x1 x2) z))).*)
+Focus 3.
+intros t' s H0.
+destruct H0 as [H0a H0b] using (glue_eq_ind Xeq).
+simpl.
+apply Split_ind.
+apply StepF_eq_trans.
 
-destruct (Split y o). destruct (Split z o).
-assert (forall ss tt, (StepFfoldProp (glue o ss tt))<-> (StepFfoldProp ss/\ StepFfoldProp tt)).
- unfold StepFfoldProp. simpl. intuition.
-rewrite H. intros [H1 H2].
-(* Should be a lemma?*)
- unfold StepF_eq. simpl.
+induction s.
+ intros t t' H0.
+ simpl.
+ eapply Map_resp_StepF_eq;try apply Yst; auto with *.
+intros t t' H0.
+simpl.
+apply Split_ind.
+apply Split_ind.
+simpl.
+apply StepF_eq_aux.
+ apply SplitL_glue_ind; intros H1; try (elim (Qlt_not_le _ _ H1); auto with *).
+ apply IHs1.
+ apply SplitL_resp_Xeq; auto with *.
+apply SplitR_glue_ind; intros H1; try (elim (Qlt_not_le _ _ H1); auto with *).
+apply IHs2.
+apply SplitR_resp_Xeq; auto with *.
+Qed.
+
 
 Lemma StepF_eq_symm:forall x y : StepF X, StepF_eq x y -> StepF_eq y x.
 intro s. unfold StepF_eq. induction s. 
